@prefix rdf: <http://www.w3.org/1999/02/22-rdf-syntax-ns#>.
@prefix rdfs: <http://www.w3.org/2000/01/rdf-schema#>.
@prefix xsd: <http://www.w3.org/2001/XMLSchema#>.
@prefix dwc: <http://rs.tdwg.org/dwc/terms/>.
@prefix dwcattributes: <http://rs.tdwg.org/dwc/terms/attributes/>.
@prefix dcterms: <http://purl.org/dc/terms/>.
@prefix dcat: <http://www.w3.org/ns/dcat#>.
@prefix owl: <http://www.w3.org/2002/07/owl#>.
@prefix skos: <http://www.w3.org/2004/02/skos/core#>.
@prefix emv: <http://rs.gbif.org/vocabulary/gbif/establishment_means/>.
@prefix gts: <http://resource.geosciml.org/ontology/timescale/gts#>.
@prefix rank: <http://resource.geosciml.org/ontology/timescale/rank/>.
@prefix isc: <http://resource.geosciml.org/classifier/ics/ischart/>.

# Caveat: This document is a work in progress and has no official standing. It is subject to change at any time and should not be considered to be stable nor citable.

emv:  a skos:ConceptScheme,
        owl:Ontology;  #is this a bad thing?  That's the approach used in the draft Hierarchy Model.  It's allowed by SKOS.
        rdfs:label             "Establishment Means GBIF Vocabulary"@en ;
#       vs.
        dcterms:title          "Establishment Means GBIF Vocabulary"@en ;
#       vs.
        skos:prefLabel         "Establishment Means GBIF Vocabulary"@en;
        
        dcterms:description         "This is a controlled vocabulary intended to be used as values for dwc:establishmentMeans."@en ;
#       vs.
        skos:note                   "This is a controlled vocabulary intended to be used as values for dwc:establishmentMeans."@en ;

        dcterms:created            "2015-02-13"^^xsd:date ;
#       vs.
        dcterms:issued             "2015-02-13"^^xsd:date ;
#       vs.
        dcterms:modified           "2015-02-13"^^xsd:date ;

        dcterms:rights              <https://creativecommons.org/licenses/by/4.0/> ;
#       vs. its subproperty
        dcterms:license             <https://creativecommons.org/licenses/by/4.0/> ;

        rdfs:seeAlso <http://rs.gbif.org/vocabulary/gbif/establishment_means.xml>,
                     <http://terms.tdwg.org/wiki/>; # here is the link to the translations document
        skos:hasTopConcept emv:native,
                           emv:introduced,
                           emv:uncertain;
 
        dcterms:creator             "Global Biodiversity Information Facility and Biodiversity Information Standards"@en ;
        rdfs:isDefinedBy       <http://foo> .
      
# Note: No labels are included in this standards document.  They are included in a separate document that is not part of the standard.

emv:native skos:definition "A species that is a part of the balance of nature that has developed over hundreds or thousands of years in a particular region or ecosystem. The word native should always be used with a geographic qualifier (for example, native to New England)."@en;
# What about using rdfs:comment for term definitions as in Dublin and Darwin Cores???
           rdf:value "native";
           rdfs:label "native"@en ;  # Do we want to have a label property even if prefLabel will be specified elsewhere? This is the precedent with DwC and 
           skos:inScheme emv:;
           rdfs:isDefinedBy emv:;
           a skos:Concept.

emv:introduced skos:definition "A species introduced with human help (intentionally or accidentally) to a new place or new type of habitat where it was not previously found. Not all non-native species are invasive. In fact, when many non-native species are introduced to new places, they cannot reproduce or spread readily without continued human help (for example, many ornamental plants)."@en;
           rdf:value "introduced";
           skos:inScheme emv:;
           rdfs:isDefinedBy emv:;
           a skos:Concept.

emv:naturalised skos:definition "The organism reproduces naturally and forms part of the local ecology."@en;
           rdf:value "naturalised";
           skos:broader emv:introduced;
           skos:inScheme emv:;
           rdfs:isDefinedBy emv:;
           a skos:Concept.

emv:invasive skos:definition "The organism is having a deleterious impact on another organism, multiple organisms or the ecosystem as a whole."@en;
           rdf:value "invasive";
           skos:broader emv:introduced;
           skos:inScheme emv:;
           rdfs:isDefinedBy emv:;
           a skos:Concept.

emv:managed skos:definition "The organism maintains its presence through intentional cultivation or husbandry."@en;
           rdf:value "managed";
           skos:broader emv:introduced;
           skos:inScheme emv:;
           rdfs:isDefinedBy emv:;
           a skos:Concept.

emv:uncertain skos:definition "Origin of organism is uncertain."@en;
           rdf:value "uncertain";
           skos:inScheme emv:;
           rdfs:isDefinedBy emv:;
           a skos:Concept.

