@prefix rdf: <http://www.w3.org/1999/02/22-rdf-syntax-ns#>.
@prefix rdfs: <http://www.w3.org/2000/01/rdf-schema#>.
@prefix xsd: <http://www.w3.org/2001/XMLSchema#>.
@prefix dwc: <http://rs.tdwg.org/dwc/terms/>.
@prefix dwcattributes: <http://rs.tdwg.org/dwc/terms/attributes/>.
@prefix dcterms: <http://purl.org/dc/terms/>.
@prefix dcmitype: <http://purl.org/dc/dcmitype/>.
@prefix dcam: <http://purl.org/dc/dcam/>.
@prefix dcat: <http://www.w3.org/ns/dcat#>.
@prefix owl: <http://www.w3.org/2002/07/owl#>.
@prefix skos: <http://www.w3.org/2004/02/skos/core#>.
@prefix emv: <http://rs.gbif.org/vocabulary/gbif/establishment_means/>.
@prefix vann: <http://purl.org/vocab/vann/>.

# Caveat: This document is a work in progress and has no official standing. It is subject to change at any time and should not be considered to be stable nor citable.

<http://rs.tdwg.org/cvterms/establishment_means> a skos:ConceptScheme,
                                                   dcmitype:Dataset;
     rdfs:label "TDWG Establishment Means Vocabulary"@en;
     dcterms:title "TDWG Establishment Means Vocabulary"@en;
     rdfs:comment "This is a controlled vocabulary whose IRIs are intended to be used as values for dwciri:establishmentMeans."@en;
     dcterms:description "This is a controlled vocabulary whose IRIs are intended to be used as values for dwciri:establishmentMeans."@en;
     skos:note "This is a controlled vocabulary intended to be used as values for dwciri:establishmentMeans."@en;
     skos:hasTopConcept emv:native,
                        emv:introduced,
                        emv:uncertain;
     vann:termGroup emv:;
     dcterms:publisher "Biodiversity Information Standards"@en.
      
# Note: No SKOS labels are included in this standards document.  They are included in a separate document that is not part of the standard.

emv: a dcat:Dataset;
     rdfs:label "Establishment Means Term List"@en;
     dcterms:title "GBIF Establishment Means Term List"@en;
     rdfs:comment "This document contains definitions for controlled vocabulary terms to be used as values for dwciri:establishmentMeans."@en;
     dcterms:description "This document contains definitions for controlled vocabulary terms to be used as values for dwciri:establishmentMeans."@en;
     skos:note "This document contains definitions for controlled vocabulary terms to be used as values for dwciri:establishmentMeans."@en;
     vann:preferredNamespacePrefix "emv";
     vann:preferredNamespaceUri "http://rs.gbif.org/vocabulary/gbif/establishment_means/";
     dcterms:modified "2015-02-13"^^xsd:date;
     dcterms:license <https://creativecommons.org/licenses/by/4.0/>;
     rdfs:seeAlso <http://rs.gbif.org/vocabulary/gbif/establishment_means.xml>,
                  <http://terms.tdwg.org/wiki/>; # here is the link to the translations document
     dcterms:isPartOf <http://rs.tdwg.org/cvterms/establishment_means>;
     dcterms:publisher "Global Biodiversity Information Facility"@en.

emv:native skos:definition "A species that is a part of the balance of nature that has developed over hundreds or thousands of years in a particular region or ecosystem. The word native should always be used with a geographic qualifier (for example, native to New England)."@en;
           rdfs:comment "A species that is a part of the balance of nature that has developed over hundreds or thousands of years in a particular region or ecosystem. The word native should always be used with a geographic qualifier (for example, native to New England)."@en;
           rdf:value "native";
           rdfs:label "native"@en;
           skos:inScheme <http://rs.tdwg.org/cvterms/establishment_means>;
           rdfs:isDefinedBy emv:;
           dcterms:isPartOf emv:;
           dcam:memberOf emv:;
           a skos:Concept.

emv:introduced skos:definition "A species introduced with human help (intentionally or accidentally) to a new place or new type of habitat where it was not previously found. Not all non-native species are invasive. In fact, when many non-native species are introduced to new places, they cannot reproduce or spread readily without continued human help (for example, many ornamental plants)."@en;
           rdfs:comment "A species introduced with human help (intentionally or accidentally) to a new place or new type of habitat where it was not previously found. Not all non-native species are invasive. In fact, when many non-native species are introduced to new places, they cannot reproduce or spread readily without continued human help (for example, many ornamental plants)."@en;
           rdf:value "introduced";
           rdfs:label "introduced"@en;
           skos:inScheme <http://rs.tdwg.org/cvterms/establishment_means>;
           rdfs:isDefinedBy emv:;
           dcterms:isPartOf emv:;
           dcam:memberOf emv:;
           a skos:Concept.

emv:naturalised skos:definition "The organism reproduces naturally and forms part of the local ecology."@en;
           rdfs:comment "The organism reproduces naturally and forms part of the local ecology."@en;
           rdf:value "naturalised";
           rdfs:label "naturalised"@en;
           skos:broader emv:introduced;
           skos:inScheme <http://rs.tdwg.org/cvterms/establishment_means>;
           rdfs:isDefinedBy emv:;
           dcterms:isPartOf emv:;
           dcam:memberOf emv:;
           a skos:Concept.

emv:invasive skos:definition "The organism is having a deleterious impact on another organism, multiple organisms or the ecosystem as a whole."@en;
           rdfs:comment "The organism is having a deleterious impact on another organism, multiple organisms or the ecosystem as a whole."@en;
           rdf:value "invasive";
           rdfs:label "invasive"@en;
           skos:broader emv:introduced;
           skos:inScheme <http://rs.tdwg.org/cvterms/establishment_means>;
           rdfs:isDefinedBy emv:;
           dcterms:isPartOf emv:;
           dcam:memberOf emv:;
           a skos:Concept.

emv:managed skos:definition "The organism maintains its presence through intentional cultivation or husbandry."@en;
           rdfs:comment "The organism maintains its presence through intentional cultivation or husbandry."@en;
           rdf:value "managed";
           rdfs:label "managed"@en;
           skos:broader emv:introduced;
           skos:inScheme <http://rs.tdwg.org/cvterms/establishment_means>;
           rdfs:isDefinedBy emv:;
           dcterms:isPartOf emv:;
           dcam:memberOf emv:;
           a skos:Concept.

emv:uncertain skos:definition "Origin of organism is uncertain."@en;
           rdfs:comment "Origin of organism is uncertain."@en;
           rdf:value "uncertain";
           rdfs:label "uncertain"@en;
           skos:inScheme <http://rs.tdwg.org/cvterms/establishment_means>;
           rdfs:isDefinedBy emv:;
           dcterms:isPartOf emv:;
           dcam:memberOf emv:;
           a skos:Concept.

